src/Program.v
@@ -1,304 +1,130 @@
-Require Import Coq.Program.Tactics.
 Require Import Coq.Program.Equality.
+Require Import Coq.Program.Tactics.
 Require Import Coq.Relations.Relations.
 Require Import Coq.Setoids.Setoid.
 
-
+Require Import FreeSpec.Equiv.
 Require Import FreeSpec.TemporalLogic.
+Require Import FreeSpec.Tuple.
+Require Import FreeSpec.Interp.
+
+Local Open Scope eq_scope.
 
 Section PROGRAM.
-  Variables (Instruction: Type -> Type).
+  Variables (I: Type -> Type).
 
   Inductive Program (A: Type) :=
   | bind {B: Type}
          (p: Program B)
          (f: B -> Program A)
     : Program A
-  | instr (i: Instruction A)
+  | instr (i: I A)
     : Program A
   | ret (a: A)
     : Program A.
 
-  Section INTERP.
-    CoInductive Interp: Type :=
-    | interp (f: forall {A: Type}, Instruction A -> (A * Interp))
-      : Interp.
+  Fixpoint runProgram
+           {A: Type}
+           (p: Program A)
+           (int: Interp I)
+    : (A * (Interp I)) :=
+    match p with
+    | ret _ a => (a, int)
+    | instr _ i => interpret i int
+    | bind _ p' f => runProgram (f (fst (runProgram p' int))) (snd (runProgram p' int))
+    end.
 
-    Section DO_INTERP.
-      Definition interpret
-                 {A: Type}
-                 (int: Interp)
-                 (i: Instruction A)
-      : (A * Interp) :=
-        match int with interp f => f A i end.
+  Definition evalProgram
+             {A: Type}
+             (p: Program A)
+             (int: Interp I)
+    : A :=
+    fst (runProgram p int).
 
-      Fixpoint runProgram
-               {A: Type}
-               (int: Interp)
-               (p: Program A)
-        : (A * Interp) :=
-        match p with
-        | ret _ a => (a, int)
-        | instr _ i => interpret int i
-        | bind _ p' f => runProgram (snd (runProgram int p')) (f (fst (runProgram int p')))
-        end.
-    End DO_INTERP.
+  Definition execProgram
+             {A: Type}
+             (p: Program A)
+             (int: Interp I)
+    : Interp I :=
+    snd (runProgram p int).
 
-    CoInductive interp_eq
-                (i1: Interp)
-                (i2: Interp)
-      : Prop :=
-    | interp_is_eq (Hres: forall {A: Type}
-                                 {p: Instruction A},
-                       fst (interpret i1 p) = fst (interpret i2 p))
-                   (Hnext: forall {A: Type}
-                                  {p: Instruction A},
-                       interp_eq (snd (interpret i1 p)) (snd (interpret i2 p)))
-      : interp_eq i1 i2.
+  CoInductive program_eq
+              (i: Interp I)
+              {A: Type}
+              `{Eq A}
+              (p: Program A)
+              (p': Program A) :=
+  | program_is_eq (Hres: evalProgram p i == evalProgram p' i)
+                  (Hnext: execProgram p i == execProgram p' i)
+    : program_eq i p p'.
 
-    Lemma interp_eq_refl
-      : forall (i: Interp), interp_eq i i.
-    Proof.
-      cofix.
-      intro i.
-      constructor.
-      + reflexivity.
-      + intros A p.
-        apply interp_eq_refl.
-    Qed.
+  Lemma program_eq_refl
+        (i: Interp I)
+    : forall {A: Type}
+             `{Eq A}
+             (p: Program A),
+      program_eq i p p.
+  Proof.
+    intros A eqA p; constructor; reflexivity.
+  Qed.
 
-    Lemma interp_eq_sym
-      : forall (i i': Interp), interp_eq i i' -> interp_eq i' i.
-    Proof.
-      cofix.
-      intros i i' H1.
-      destruct H1.
-      constructor.
-      + intros A p.
-        symmetry.
-        exact (Hres A p).
-      + intros A p.
-        apply (interp_eq_sym (snd (interpret i p)) (snd (interpret i' p)) (Hnext A p)).
-    Qed.
+  Lemma program_eq_sym
+        (i: Interp I)
+    : forall {A: Type}
+             `{Eq A}
+             (p p': Program A),
+      program_eq i p p'
+      -> program_eq i p' p.
+  Proof.
+    intros A eqA p p' H1.
+    destruct H1 as [Hres Hnext].
+    constructor; symmetry; assumption.
+  Qed.
 
-    Lemma interp_eq_trans
-      : forall (i i' i'': Interp),
-        interp_eq i i'
-        -> interp_eq i' i''
-        -> interp_eq i i''.
-    Proof.
-      cofix.
-      intros i i' i'' H1 H2.
-      destruct H1 as [Hres1 Hnext1].
-      destruct H2 as [Hres2 Hnext2].
-      constructor.
-      + intros A p.
-        rewrite <- (Hres2 A p).
-        exact (Hres1 A p).
-      + intros A p.
-        apply (interp_eq_trans (snd (interpret i p))
-                               (snd (interpret i' p))
-                               (snd (interpret i'' p))
-                               (Hnext1 A p)
-                               (Hnext2 A p)).
-    Qed.
+  Lemma program_eq_trans
+        (i: Interp I)
+    : forall {A: Type}
+             `{Eq A}
+             (p p' p'': Program A),
+      program_eq i p p'
+      -> program_eq i p' p''
+      -> program_eq i p p''.
+  Proof.
+    intros A eqA p p' p'' [Hres1 Hnext1] [Hres2 Hnext2].
+    constructor.
+    + transitivity (evalProgram p' i); assumption.
+    + transitivity (execProgram p' i); assumption.
+  Qed.
 
-    Add Parametric Relation : (Interp) (interp_eq)
-      reflexivity proved by (interp_eq_refl)
-      symmetry proved by (interp_eq_sym)
-      transitivity proved by (interp_eq_trans)
-        as interp_rel.
+  Add Parametric Relation
+      (int: Interp I)
+      (A: Type)
+      (eqA: Eq A)
+    : (Program A) (@program_eq int A eqA)
+      reflexivity proved by (@program_eq_refl int A eqA)
+      symmetry proved by (@program_eq_sym int A eqA)
+      transitivity proved by (@program_eq_trans int A eqA)
+        as program_rel.
 
-    Require Import Morphisms.
+  Definition interp_assoc
+             (int: Interp I)
+    := forall {A B C: Type}
+              `{Eq C}
+              (p: Program A)
+              (f: A -> Program B)
+              (g: B -> Program C),
+      program_eq int (bind _ (bind _ p f) g) (bind _ p (fun x => bind _ (f x) g)).
 
-    Definition interp_ret_eq
-               {A: Type}
-               (x: (A * Interp))
-               (y: (A * Interp))
-      : Prop :=
-      fst x = fst y /\ interp_eq (snd x) (snd y).
+  Definition interp_assoc2
+             (int: Interp I)
+    := forall {A B: Type}
+              `{Eq B}
+              (p: Program A)
+              (f: A -> Program B),
+      evalProgram (bind B p f) int
+      == evalProgram (f (evalProgram p int)) (execProgram p int).
 
-    Lemma interp_ret_eq_refl
-          {A: Type}
-          (x: (A * Interp))
-      : interp_ret_eq x x.
-    Proof.
-      split; reflexivity.
-    Qed.
-
-    Lemma interp_ret_eq_sym
-          {A: Type}
-          (x: (A * Interp))
-          (y: (A * Interp))
-      : interp_ret_eq x y -> interp_ret_eq y x.
-    Proof.
-      intros [H1 H2].
-      split; symmetry; assumption.
-    Qed.
-
-    Lemma interp_ret_eq_trans
-          {A: Type}
-          (x: (A * Interp))
-          (y: (A * Interp))
-          (z: (A * Interp))
-      : interp_ret_eq x y
-        -> interp_ret_eq y z
-        -> interp_ret_eq x z.
-    Proof.
-      intros [H1 H2] [H1' H2'].
-      split.
-      + transitivity (fst y); assumption.
-      + transitivity (snd y); assumption.
-    Qed.
-
-    Add Parametric Relation (A: Type) : (A * Interp) (@interp_ret_eq A)
-      reflexivity proved by (interp_ret_eq_refl)
-      symmetry proved by (interp_ret_eq_sym)
-      transitivity proved by (interp_ret_eq_trans)
-        as interp_ret_rel.
-
-    Add Parametric Morphism
-        (A: Type): (@snd A Interp)
-        with signature (@interp_ret_eq A) ==> (interp_eq)
-          as snd_interp_ret.
-    Proof.
-      intros [a int] [b int'] [Heq1 Heq2].
-      exact Heq2.
-    Qed.
-
-    Add Parametric Morphism
-        (A: Type): (@fst A Interp)
-        with signature (@interp_ret_eq A) ==> (@eq A)
-          as fst_interp_ret.
-    Proof.
-      intros [a int] [b int'] [Heq1 Heq2].
-      exact Heq1.
-    Qed.
-
-    Add Parametric Morphism
-        (A: Type) (i: Instruction A): (fun int => snd (interpret int i))
-        with signature (@interp_eq) ==> (@interp_eq)
-          as interp_morph.
-    Proof.
-      intros int int' Heq.
-      destruct Heq as [H1 H2].
-      apply H2.
-    Qed.
-
-    Add Parametric Morphism
-        (A: Type) (i: Instruction A): (fun int => fst (interpret int i))
-        with signature (@interp_eq) ==> (@eq A)
-          as interp_res_morph.
-    Proof.
-      intros int int' Heq.
-      destruct Heq as [H1 H2].
-      apply H1.
-    Qed.
-
-    Add Parametric Morphism
-        (A: Type) (p: Program A): (fun int => snd (runProgram int p))
-        with signature (@interp_eq) ==> (@interp_eq)
-          as runProgram_morph.
-    Proof.
-      intros int int' Heq.
-      induction p.
-      + admit.
-      + destruct Heq as [H1 H2];
-          cbn;
-          apply H2.
-      + cbn; exact Heq.
-    Admitted.
-
-    Add Parametric Morphism
-        (A: Type) (p: Program A): (fun int => fst (runProgram int p))
-        with signature (@interp_eq) ==> (@eq A)
-          as runProgram_ret_morph.
-    Proof.
-      intros int int' Heq.
-      induction p.
-      + admit.
-      + destruct Heq as [H1 H2];
-          cbn;
-          apply H1.
-      + cbn; reflexivity.
-    Admitted.
-
-    CoInductive program_eq
-                (i: Interp)
-                {A: Type}
-                (p: Program A)
-                (p': Program A) :=
-    | program_is_eq (Hres: fst (runProgram i p) = fst (runProgram i p'))
-                    (Hnext: interp_eq (snd (runProgram i p)) (snd (runProgram i p'))): program_eq i p p'.
-
-    Lemma program_eq_refl
-          (i: Interp)
-      : forall {A: Type} (p: Program A), program_eq i p p.
-    Proof.
-      intro A.
-      cofix.
-      intro p.
-      constructor.
-      + reflexivity.
-      + apply interp_eq_refl.
-    Qed.
-
-    Lemma program_eq_sym
-          (i: Interp)
-      : forall {A: Type}
-               (p p': Program A),
-        program_eq i p p'
-        -> program_eq i p' p.
-    Proof.
-      intro A.
-      cofix.
-      intros p p' H1.
-      destruct H1 as [Hres Hnext].
-      constructor.
-      + symmetry; exact Hres.
-      + apply (interp_eq_sym (snd (runProgram i p))
-                             (snd (runProgram i p'))
-                             Hnext).
-    Qed.
-
-    Lemma program_eq_trans
-          (i: Interp)
-      : forall {A: Type}
-               (p p' p'': Program A),
-        program_eq i p p'
-        -> program_eq i p' p''
-        -> program_eq i p p''.
-    Proof.
-      intro A.
-      cofix.
-      intros p p' p'' [Hres1 Hnext1] [Hres2 Hnext2].
-      constructor.
-      + rewrite <- Hres2; exact Hres1.
-      + apply (interp_eq_trans (snd (runProgram i p))
-                               (snd (runProgram i p'))
-                               (snd (runProgram i p''))
-                               Hnext1
-                               Hnext2).
-    Qed.
-
-    Definition interp_assoc
-               (int: Interp)
-      := forall {A B C: Type}
-                (p: Program A)
-                (f: A -> Program B)
-                (g: B -> Program C),
-        program_eq int (bind _ (bind _ p f) g) (bind _ p (fun x => bind _ (f x) g)).
-
-    Definition interp_assoc2
-               (int: Interp)
-      := forall {A B: Type}
-                (p: Program A)
-                (f: A -> Program B),
-        fst (runProgram int (bind _ p f))
-        = fst (runProgram (snd (runProgram int p)) (f (fst (runProgram int p)))).
-
-  End INTERP.
-
+  (*
   Section TL.
     Inductive ISet: Type :=
     | instruction {A: Type}
@@ -320,43 +146,58 @@ Section PROGRAM.
                              (f (fst (fst (runTL int p' tl))))
                              (snd (runTL int p' tl))
       end.
+
+    Lemma run_tl_run_program_interp_eq
+          {A: Type}
+      : forall (p: Program A)
+               (tl: TL (ISet))
+               (int: Interp),
+        interp_eq (snd (fst (runTL int p tl))) (snd (runProgram int p)).
+    Proof.
+      cofix.
+      induction p.
+      + admit.
+      + cbn.
+        intros tl int.
+    Admitted.
   End TL.
+  *)
 
   Section CONTRACT.
     Definition typeret
                {A: Type}
-               (i: Instruction A)
+               (i: I A)
     : Type := A.
 
     Record Contract :=
       { requirements {A: Type}
-                     (i: Instruction A)
+                     (i: I A)
         : Prop
       ; promises {A: Type}
-                 (i: Instruction A)
+                   (i: I A)
         : typeret i -> Prop
-     }.
+      }.
 
     Variable (c: Contract).
 
     CoInductive Enforcer
-                (int: Interp)
+                (int: Interp I)
       : Prop :=
     | enforced (Hprom: forall {A: Type}
-                              (i: Instruction A),
+                              (i: I A),
                    requirements c i
-                   -> (promises c i) (fst (interpret int i)))
+                   -> (promises c i) (evalInstruction i int))
                (Henf:  forall {A: Type}
-                              (i: Instruction A),
+                              (i: I A),
                    requirements c i
-                   -> Enforcer (snd (interpret int i)))
+                   -> Enforcer (execInstruction i int))
       : Enforcer int.
 
     Section PROGRAM_CONTRACT.
       Inductive contractfull_program
         : forall {A: Type}, Program A -> Type :=
       | contractfull_instr {A: Type}
-                           (i: Instruction A)
+                           (i: I A)
                            (Hreq: requirements c i)
         : contractfull_program (instr A i)
       | contractfull_ret {A: Type}
@@ -366,21 +207,20 @@ Section PROGRAM.
                          (p: Program A)
                          (f: A -> Program B)
                          (Hcp: contractfull_program p)
-                         (Hnext: forall (int: Interp)
+                         (Hnext: forall (int: Interp I)
                                         (Henf: Enforcer int),
-                             contractfull_program (f (fst (runProgram int p))))
+                             contractfull_program (f (evalProgram p int)))
         : contractfull_program (bind B p f).
 
       Lemma contractfull_instr_enforcement
             {A: Type}
-            (i: Instruction A)
-        : forall (int: Interp),
+            (i: I A)
+        : forall (int: Interp I),
           contractfull_program (instr A i)
           -> Enforcer int
-          -> Enforcer (snd (runProgram int (instr A i))).
+          -> Enforcer (execProgram (instr A i) int).
       Proof.
         intros int Hc Henf.
-        cbn in *.
         destruct Henf as [Hprom Henf].
         apply (Henf A i).
         inversion Hc; simpl_existT; subst.
@@ -390,34 +230,32 @@ Section PROGRAM.
       Lemma contractfull_ret_enforcement
             {A: Type}
             (a: A)
-        : forall (int: Interp),
+        : forall (int: Interp I),
           contractfull_program (ret A a)
           -> Enforcer int
-          -> Enforcer (snd (runProgram int (ret A a))).
+          -> Enforcer (execProgram (ret A a) int).
       Proof.
         intros int Hc Henf.
-        cbn in *.
         exact Henf.
       Qed.
 
       Lemma contractfull_program_enforcement
             {A B: Type}
             (p: Program A)
-        : forall (int: Interp),
+        : forall (int: Interp I),
           contractfull_program p
           -> Enforcer int
-          -> Enforcer (snd (runProgram int p)).
+          -> Enforcer (execProgram p int).
       Proof.
         induction p.
         + intros int Hc Henf.
-          assert (contractfull_program (f (fst (runProgram int p)))) as Hc'.
-          * inversion Hc; repeat simpl_existT; subst.
-            apply (Hnext int Henf).
-          * inversion Hc; repeat simpl_existT; subst.
-            apply H with (int:=snd (runProgram int p)) in Hc'.
-            cbn.
-            exact Hc'.
-            apply IHp; [ exact Hcp
+          assert (contractfull_program (f (evalProgram p int))) as Hc'.
+          ++ inversion Hc; repeat simpl_existT; subst.
+             apply (Hnext int Henf).
+          ++ inversion Hc; repeat simpl_existT; subst.
+             apply H with (int := execProgram p int) in Hc'.
+             exact Hc'.
+             apply IHp; [ exact Hcp
                        | exact Henf
                        ].
         + apply contractfull_instr_enforcement.
@@ -430,15 +268,15 @@ Section PROGRAM.
     Variables (State: Type).
 
     Definition PS
-      := forall {A: Type}, State -> Instruction A -> (A * State).
+      := forall {A: Type}, State -> I A -> (A * State).
 
     CoFixpoint mkInterp
                (ps: PS)
                (s: State)
-      : Interp :=
+      : Interp I :=
       interp (
           fun (A: Type)
-              (p: Instruction A) =>
+              (p: I A) =>
             (fst  (ps A s p), mkInterp ps (snd (ps A s p)))).
 
     Lemma mkInterp_is_assoc
@@ -468,7 +306,7 @@ Section PROGRAM.
 
       Definition contract_preserves_inv
         := forall {A: Type}
-                  (i: Instruction A)
+                  (i: I A)
                   (s: State),
            inv s
            -> requirements c i
@@ -476,7 +314,7 @@ Section PROGRAM.
 
       Definition contract_enforces_promises
         := forall {A: Type}
-                  (i: Instruction A)
+                  (i: I A)
                   (s: State),
           inv s
           -> requirements c i
@@ -492,30 +330,31 @@ Section PROGRAM.
         split; intros A i Hreq; cbn.
         + apply (Henf A i s Hinv Hreq).
         + apply (Hpres A i s) in Hinv.
-          - apply (stateful_contract_enforcement  (snd (step A s i)) Hinv).
-          - exact Hreq.
+          ++ apply (stateful_contract_enforcement  (snd (step A s i)) Hinv).
+          ++ exact Hreq.
       Qed.
     End STATEFUL_INTERP_ENFORCER.
   End MAKE_INTERP.
 End PROGRAM.
 
-Arguments bind [Instruction A B] (p f).
-Arguments instr [Instruction A] (i).
-Arguments ret [Instruction A] (a).
+Arguments bind [I A B] (p f).
+Arguments instr [I A] (i).
+Arguments ret [I A] (a).
 
-Arguments mkInterp [Instruction State] (ps s).
+Arguments mkInterp [I State] (ps s).
 
-Arguments interpret [Instruction A] (int i).
-Arguments runProgram [Instruction A] (int p).
+Arguments runProgram [I A] (p int).
+Arguments execProgram [I A] (p int).
+Arguments evalProgram [I A] (p int).
 
-Arguments typeret [Instruction A] (i).
-Arguments Enforcer [Instruction] (c int).
+Arguments typeret [I A] (i).
+Arguments Enforcer [I] (c int).
 
-Arguments stateful_contract_enforcement [Instruction State] (step inv c Hpres Henf s).
-Arguments contract_enforces_promises [Instruction State] (step inv c).
-Arguments contract_preserves_inv [Instruction State] (step inv c).
+Arguments stateful_contract_enforcement [I State] (step inv c Hpres Henf s).
+Arguments contract_enforces_promises [I State] (step inv c).
+Arguments contract_preserves_inv [I State] (step inv c).
 
-Arguments contractfull_program [Instruction] c [A].
+Arguments contractfull_program [I] c [A].
 
 Notation "int <· p" := (fst (runProgram int p)) (at level 50) : prog_scope.
 Notation "p >>= f" := (bind p f) (at level 50) : prog_scope.
