src/Interp.v
@@ -1,0 +1,211 @@
+Require Import Coq.Classes.Equivalence.
+Require Import Coq.Setoids.Setoid.
+
+Require Import FreeSpec.Tuple.
+Require Import FreeSpec.Equiv.
+
+Local Open Scope eq_scope.
+
+Section INTERP.
+  Variable (Instruction: Type -> Type).
+
+  CoInductive Interp: Type :=
+  | interp (f: forall {A: Type}, Instruction A -> (A * Interp))
+    : Interp.
+
+  Definition interpret
+             {A: Type}
+             (i: Instruction A)
+             (int: Interp)
+    : (A * Interp) :=
+    match int with interp f => f A i end.
+
+  Definition evalInstruction
+             {A: Type}
+             (i: Instruction A)
+             (int: Interp)
+    : A :=
+    fst (interpret i int).
+
+  Definition execInstruction
+             {A: Type}
+             (i: Instruction A)
+             (int: Interp)
+    : Interp :=
+    snd (interpret i int).
+
+  CoInductive interp_eq
+              (i1: Interp)
+              (i2: Interp)
+    : Prop :=
+  | interp_is_eq (Hres: forall {A: Type}
+                              `{Eq A}
+                               (i: Instruction A),
+                     evalInstruction i i1 == evalInstruction i i2)
+                 (Hnext: forall {A: Type}
+                                (i: Instruction A),
+                     interp_eq (execInstruction i i1) (execInstruction i i2))
+    : interp_eq i1 i2.
+
+  Lemma interp_eq_refl
+    : forall (i: Interp), interp_eq i i.
+  Proof.
+    cofix.
+    intro i.
+    constructor.
+    + reflexivity.
+    + intros A p.
+      apply interp_eq_refl.
+  Qed.
+
+  Lemma interp_eq_sym
+    : forall (i i': Interp), interp_eq i i' -> interp_eq i' i.
+  Proof.
+    cofix.
+    intros int int' H1.
+    destruct H1.
+    constructor.
+    + intros A eqA i.
+      symmetry.
+      exact (Hres A eqA i).
+    + intros A i.
+      apply (interp_eq_sym (snd (interpret i int)) (snd (interpret i int')) (Hnext A i)).
+  Qed.
+
+  Lemma interp_eq_trans
+    : forall (i i' i'': Interp),
+      interp_eq i i'
+      -> interp_eq i' i''
+      -> interp_eq i i''.
+  Proof.
+    cofix.
+    intros i i' i'' H1 H2.
+    destruct H1 as [Hres1 Hnext1].
+    destruct H2 as [Hres2 Hnext2].
+    constructor.
+    + intros A eqA p.
+      transitivity (fst (interpret p i')).
+      exact (Hres1 A eqA p).
+      exact (Hres2 A eqA p).
+    + intros A p.
+      apply (interp_eq_trans (snd (interpret p i))
+                             (snd (interpret p i'))
+                             (snd (interpret p i''))
+                             (Hnext1 A p)
+                             (Hnext2 A p)).
+  Qed.
+End INTERP.
+
+Arguments interp [_].
+Arguments interp_eq [_].
+Arguments interpret [_ _].
+Arguments evalInstruction [_ _].
+Arguments execInstruction [_ _].
+Arguments interp_eq_refl [_].
+Arguments interp_eq_sym [_].
+Arguments interp_eq_trans [_].
+
+Add Parametric Relation
+    (I: Type -> Type)
+  : (Interp I) (@interp_eq I)
+  reflexivity proved by (@interp_eq_refl I)
+  symmetry proved by (@interp_eq_sym I)
+  transitivity proved by (@interp_eq_trans I)
+    as interp_rel.
+
+Instance eqInterp (I: Type -> Type): Eq (Interp I) :=
+  {| equiv := @interp_eq I |}.
+
+Local Open Scope eq_scope.
+
+Lemma _interp_int_morphism
+  : forall (I: Type -> Type)
+           (x y : Interp I)
+           (A: Type)
+           {eqA: Eq A}
+           (i: I A),
+  x == y -> (interpret i x) == (interpret i y).
+Proof.
+  intros I int int' A eqA i Heq.
+  constructor.
+  + destruct Heq.
+    apply (Hres A eqA i).
+  + destruct Heq.
+    assert (interp_eq (snd (interpret i int)) (snd (interpret i int')))
+      as Hin
+        by (apply Hnext).
+    apply Hnext.
+Qed.
+
+Add Parametric Morphism
+    (I: Type -> Type)
+    (A: Type)
+    (eqA: Eq A)
+    (i: I A)
+  : (interpret i)
+    with signature (@interp_eq I) ==> (@tuple_eq A (Interp I) eqA (eqInterp I))
+      as interp_int_morphism.
+Proof.
+  intros int int' Heq.
+  constructor.
+  + destruct Heq.
+    apply (Hres A eqA i).
+  + destruct Heq.
+    assert (interp_eq (snd (interpret i int)) (snd (interpret i int'))).
+    apply (Hnext A i).
+    rewrite H.
+    reflexivity.
+Qed.
+
+Add Parametric Morphism
+    (I: Type -> Type)
+    (A: Type)
+    (eqA: Eq A)
+    (i: I A)
+  : (evalInstruction i)
+    with signature (@interp_eq I) ==> (@equiv A eqA)
+      as eval_instr_morphism.
+Proof.
+  apply interp_int_morphism.
+Qed.
+
+Add Parametric Morphism
+    (I: Type -> Type)
+    (A: Type)
+    (eqA: Eq A)
+    (i: I A)
+  : (execInstruction i)
+    with signature (@interp_eq I) ==> (@interp_eq I)
+      as exec_instr_morphism.
+Proof.
+  apply interp_int_morphism.
+  exact eqA.
+Qed.
+
+(* A list of goal to check the rewrite tactic actually works *)
+
+Goal (forall (I: Type -> Type)
+             (int int': Interp I)
+             (A: Type)
+             (eqA: Eq A)
+             (i: I A),
+         int == int'
+         -> evalInstruction i int == evalInstruction i int').
+Proof.
+  intros I int int' A eqA i Heq.
+  rewrite Heq.
+  reflexivity.
+Qed.
+
+Goal (forall (I: Type -> Type)
+             (int int': Interp I)
+             (A: Type)
+             (eqA: Eq A)
+             (i: I A),
+         int == int'
+         -> execInstruction i int == execInstruction i int').
+Proof.
+  intros I int int' A eqA i Heq.
+  rewrite Heq.
+  reflexivity.
+Qed.
